Rename Opcode to Instruction

theories/Machine/Coding.v
@@ -95,48 +95,48 @@ Module TinyRAMCoding (Params : TinyRAMParameters).
     f_equal; apply proof_irrelevance.
   Qed.
 
-  Variant OpcodeI : Type :=
-  | andI : regId -> regId -> OpcodeI
-  | orI : regId -> regId -> OpcodeI
-  | xorI : regId -> regId -> OpcodeI
-  | notI : regId -> OpcodeI
-  | addI : regId -> regId -> OpcodeI
-  | subI : regId -> regId -> OpcodeI
-  | mullI : regId -> regId -> OpcodeI
-  | umulhI : regId -> regId -> OpcodeI
-  | smulhI : regId -> regId -> OpcodeI
-  | udivI : regId -> regId -> OpcodeI
-  | umodI : regId -> regId -> OpcodeI
-  | shlI : regId -> regId -> OpcodeI
-  | shrI : regId -> regId -> OpcodeI
-  | cmpeI : regId -> OpcodeI
-  | cmpaI : regId -> OpcodeI
-  | cmpaeI : regId -> OpcodeI
-  | cmpgI : regId -> OpcodeI
-  | cmpgeI : regId -> OpcodeI
-  | movI : regId -> OpcodeI
-  | cmovI : regId -> OpcodeI
-  | jmpI : OpcodeI
-  | cjmpI : OpcodeI
-  | cnjmpI : OpcodeI
-  | store_bI : regId -> OpcodeI
-  | load_bI : regId -> OpcodeI
-  | store_wI : regId -> OpcodeI
-  | load_wI : regId -> OpcodeI
-  | readI : regId -> OpcodeI
-  | answerI : OpcodeI.
+  Variant InstructionI : Type :=
+  | andI : regId -> regId -> InstructionI
+  | orI : regId -> regId -> InstructionI
+  | xorI : regId -> regId -> InstructionI
+  | notI : regId -> InstructionI
+  | addI : regId -> regId -> InstructionI
+  | subI : regId -> regId -> InstructionI
+  | mullI : regId -> regId -> InstructionI
+  | umulhI : regId -> regId -> InstructionI
+  | smulhI : regId -> regId -> InstructionI
+  | udivI : regId -> regId -> InstructionI
+  | umodI : regId -> regId -> InstructionI
+  | shlI : regId -> regId -> InstructionI
+  | shrI : regId -> regId -> InstructionI
+  | cmpeI : regId -> InstructionI
+  | cmpaI : regId -> InstructionI
+  | cmpaeI : regId -> InstructionI
+  | cmpgI : regId -> InstructionI
+  | cmpgeI : regId -> InstructionI
+  | movI : regId -> InstructionI
+  | cmovI : regId -> InstructionI
+  | jmpI : InstructionI
+  | cjmpI : InstructionI
+  | cnjmpI : InstructionI
+  | store_bI : regId -> InstructionI
+  | load_bI : regId -> InstructionI
+  | store_wI : regId -> InstructionI
+  | load_wI : regId -> InstructionI
+  | readI : regId -> InstructionI
+  | answerI : InstructionI.
 
   Definition operand : Type := Word + regId.
 
-  Definition Opcode : Type := OpcodeI * operand.
+  Definition Instruction : Type := InstructionI * operand.
 
-  Definition ijTr (con : regId -> regId -> OpcodeI)
-                   (ri rj : regId) (A : operand) : Opcode := (con ri rj, A).
+  Definition ijTr (con : regId -> regId -> InstructionI)
+                   (ri rj : regId) (A : operand) : Instruction := (con ri rj, A).
 
-  Definition iTr (con : regId -> OpcodeI)
-                   (ri : regId) (A : operand) : Opcode := (con ri, A).
+  Definition iTr (con : regId -> InstructionI)
+                   (ri : regId) (A : operand) : Instruction := (con ri, A).
 
-  Definition Tr (con : OpcodeI) (A : operand) : Opcode := (con, A).
+  Definition Tr (con : InstructionI) (A : operand) : Instruction := (con, A).
 
   Definition oreg {n} (v : Vector.t bool n) : option regId.
     destruct (bitvector_fin_big v).
@@ -223,7 +223,7 @@ Module TinyRAMCoding (Params : TinyRAMParameters).
     exact lt.
   Qed.
 
-  Definition answer1 : Opcode.
+  Definition answer1 : Instruction.
     split.
     - apply answerI.
     - apply inl, fin_bitvector_big.
@@ -244,10 +244,10 @@ Module TinyRAMCoding (Params : TinyRAMParameters).
      a word into a register address, which may be too big
      anyway.
   *)
-  Definition OpcodeDecodeA : forall
-    (code : operand -> Opcode)
+  Definition InstructionDecodeA : forall
+    (code : operand -> Instruction)
     (isReg : bool) (w2: Word) (w2reg: option regId),
-    Opcode.
+    Instruction.
     intros code isReg w2 w2reg.
     destruct isReg.
     + exact (code (inl w2)).
@@ -255,11 +255,11 @@ Module TinyRAMCoding (Params : TinyRAMParameters).
       exact (code (inr w2reg)).
   Defined.
 
-  Definition OpcodeDecodeRiA : forall
-    (code : regId -> operand -> Opcode)
+  Definition InstructionDecodeRiA : forall
+    (code : regId -> operand -> Instruction)
     (isReg : bool) (ri : option regId)
     (w2: Word) (w2reg: option regId),
-    Opcode.
+    Instruction.
     intros code isReg ri w2 w2reg.
     destruct ri as [ri|]. 2: { exact answer1. }
     destruct isReg.
@@ -268,11 +268,11 @@ Module TinyRAMCoding (Params : TinyRAMParameters).
       exact (code ri (inr w2reg)).
   Defined.
 
-  Definition OpcodeDecodeRiRjA : forall
-    (code : regId -> regId -> operand -> Opcode)
+  Definition InstructionDecodeRiRjA : forall
+    (code : regId -> regId -> operand -> Instruction)
     (isReg : bool) (ri rj : option regId)
     (w2: Word) (w2reg: option regId),
-    Opcode.
+    Instruction.
     intros code isReg ri rj w2 w2reg.
     destruct ri as [ri|]. 2: { exact answer1. }
     destruct rj as [rj|]. 2: { exact answer1. }
@@ -293,45 +293,45 @@ Module TinyRAMCoding (Params : TinyRAMParameters).
               (which is the maximum between the length of a register name
               and of an immediate value).
   """*)
-  Definition OpcodeDecode (w1 w2 : Word) : Opcode :=
+  Definition InstructionDecode (w1 w2 : Word) : Instruction :=
     match interpSplit w1 with
     | (op, isReg, pri, prj, _) =>
       let ri := oreg pri in
       let rj := oreg prj in
       let ow := oreg w2 in
       match proj1_sig (bitvector_fin_big op) with
-      | 0 =>  OpcodeDecodeRiRjA (ijTr andI  ) isReg ri rj w2 ow
-      | 1 =>  OpcodeDecodeRiRjA (ijTr orI   ) isReg ri rj w2 ow
-      | 2 =>  OpcodeDecodeRiRjA (ijTr xorI  ) isReg ri rj w2 ow
-      | 3 =>  OpcodeDecodeRiA   (iTr  notI  ) isReg ri w2 ow
-      | 4 =>  OpcodeDecodeRiRjA (ijTr addI  ) isReg ri rj w2 ow
-      | 5 =>  OpcodeDecodeRiRjA (ijTr subI  ) isReg ri rj w2 ow
-      | 6 =>  OpcodeDecodeRiRjA (ijTr mullI ) isReg ri rj w2 ow
-      | 7 =>  OpcodeDecodeRiRjA (ijTr umulhI) isReg ri rj w2 ow
-      | 8 =>  OpcodeDecodeRiRjA (ijTr smulhI) isReg ri rj w2 ow
-      | 9 =>  OpcodeDecodeRiRjA (ijTr udivI ) isReg ri rj w2 ow
-      | 10 => OpcodeDecodeRiRjA (ijTr umodI ) isReg ri rj w2 ow
-      | 11 => OpcodeDecodeRiRjA (ijTr shlI  ) isReg ri rj w2 ow
-      | 12 => OpcodeDecodeRiRjA (ijTr shrI  ) isReg ri rj w2 ow
-      | 13 => OpcodeDecodeRiA   (iTr  cmpeI ) isReg rj w2 ow
-      | 14 => OpcodeDecodeRiA   (iTr  cmpaI ) isReg rj w2 ow
-      | 15 => OpcodeDecodeRiA   (iTr  cmpaeI) isReg rj w2 ow
-      | 16 => OpcodeDecodeRiA   (iTr  cmpgI ) isReg rj w2 ow
-      | 17 => OpcodeDecodeRiA   (iTr  cmpgeI) isReg rj w2 ow
-      | 18 => OpcodeDecodeRiA   (iTr  movI  ) isReg ri w2 ow
-      | 19 => OpcodeDecodeRiA   (iTr  cmovI ) isReg ri w2 ow
-      | 20 => OpcodeDecodeA     (Tr   jmpI  ) isReg w2 ow
-      | 21 => OpcodeDecodeA     (Tr   cjmpI ) isReg w2 ow
-      | 22 => OpcodeDecodeA     (Tr   cnjmpI) isReg w2 ow
+      | 0 =>  InstructionDecodeRiRjA (ijTr andI  ) isReg ri rj w2 ow
+      | 1 =>  InstructionDecodeRiRjA (ijTr orI   ) isReg ri rj w2 ow
+      | 2 =>  InstructionDecodeRiRjA (ijTr xorI  ) isReg ri rj w2 ow
+      | 3 =>  InstructionDecodeRiA   (iTr  notI  ) isReg ri w2 ow
+      | 4 =>  InstructionDecodeRiRjA (ijTr addI  ) isReg ri rj w2 ow
+      | 5 =>  InstructionDecodeRiRjA (ijTr subI  ) isReg ri rj w2 ow
+      | 6 =>  InstructionDecodeRiRjA (ijTr mullI ) isReg ri rj w2 ow
+      | 7 =>  InstructionDecodeRiRjA (ijTr umulhI) isReg ri rj w2 ow
+      | 8 =>  InstructionDecodeRiRjA (ijTr smulhI) isReg ri rj w2 ow
+      | 9 =>  InstructionDecodeRiRjA (ijTr udivI ) isReg ri rj w2 ow
+      | 10 => InstructionDecodeRiRjA (ijTr umodI ) isReg ri rj w2 ow
+      | 11 => InstructionDecodeRiRjA (ijTr shlI  ) isReg ri rj w2 ow
+      | 12 => InstructionDecodeRiRjA (ijTr shrI  ) isReg ri rj w2 ow
+      | 13 => InstructionDecodeRiA   (iTr  cmpeI ) isReg rj w2 ow
+      | 14 => InstructionDecodeRiA   (iTr  cmpaI ) isReg rj w2 ow
+      | 15 => InstructionDecodeRiA   (iTr  cmpaeI) isReg rj w2 ow
+      | 16 => InstructionDecodeRiA   (iTr  cmpgI ) isReg rj w2 ow
+      | 17 => InstructionDecodeRiA   (iTr  cmpgeI) isReg rj w2 ow
+      | 18 => InstructionDecodeRiA   (iTr  movI  ) isReg ri w2 ow
+      | 19 => InstructionDecodeRiA   (iTr  cmovI ) isReg ri w2 ow
+      | 20 => InstructionDecodeA     (Tr   jmpI  ) isReg w2 ow
+      | 21 => InstructionDecodeA     (Tr   cjmpI ) isReg w2 ow
+      | 22 => InstructionDecodeA     (Tr   cnjmpI) isReg w2 ow
       | 23 => answer1
       | 24 => answer1
       | 25 => answer1
-      | 26 => OpcodeDecodeRiA (iTr   store_bI) isReg ri w2 ow
-      | 27 => OpcodeDecodeRiA (iTr   load_bI ) isReg ri w2 ow
-      | 28 => OpcodeDecodeRiA (iTr   store_wI) isReg ri w2 ow
-      | 29 => OpcodeDecodeRiA (iTr   load_wI ) isReg ri w2 ow
-      | 30 => OpcodeDecodeRiA (iTr   readI   ) isReg ri w2 ow
-      | 31 => OpcodeDecodeA   (Tr    answerI ) isReg w2 ow
+      | 26 => InstructionDecodeRiA (iTr   store_bI) isReg ri w2 ow
+      | 27 => InstructionDecodeRiA (iTr   load_bI ) isReg ri w2 ow
+      | 28 => InstructionDecodeRiA (iTr   store_wI) isReg ri w2 ow
+      | 29 => InstructionDecodeRiA (iTr   load_wI ) isReg ri w2 ow
+      | 30 => InstructionDecodeRiA (iTr   readI   ) isReg ri w2 ow
+      | 31 => InstructionDecodeA   (Tr    answerI ) isReg w2 ow
       | _ => answer1
       end
     end.
@@ -342,56 +342,56 @@ Module TinyRAMCoding (Params : TinyRAMParameters).
 
   Ltac rirjAProof_register :=
     intros ri rj lti ltj A ltA padding;
-    unfold OpcodeDecode; rewrite interpSplit_eval;
+    unfold InstructionDecode; rewrite interpSplit_eval;
     unfold bitvector_fin_big; vector_simp; simpl;
     rewrite (regFitProp ri lti), (regFitProp rj ltj), (regFitProp A ltA);
     reflexivity.
 
   Ltac rirjAProof_word :=
     intros ri rj lti ltj A padding;
-    unfold OpcodeDecode; rewrite interpSplit_eval;
+    unfold InstructionDecode; rewrite interpSplit_eval;
     unfold bitvector_fin_big; vector_simp; simpl;
     rewrite (regFitProp ri lti), (regFitProp rj ltj);
     reflexivity.
 
   Ltac riAProof_register :=
     intros ri pad lti A ltA padding;
-    unfold OpcodeDecode; rewrite interpSplit_eval;
+    unfold InstructionDecode; rewrite interpSplit_eval;
     unfold bitvector_fin_big; vector_simp; simpl;
     rewrite (regFitProp ri lti), (regFitProp A ltA);
     reflexivity.
 
   Ltac riAProof_word :=
     intros ri pad lti A padding;
-    unfold OpcodeDecode; rewrite interpSplit_eval;
+    unfold InstructionDecode; rewrite interpSplit_eval;
     unfold bitvector_fin_big; vector_simp; simpl;
     rewrite (regFitProp ri lti);
     reflexivity.
 
   Ltac rjAProof_register :=
     intros pad ri lti A ltA padding;
-    unfold OpcodeDecode; rewrite interpSplit_eval;
+    unfold InstructionDecode; rewrite interpSplit_eval;
     unfold bitvector_fin_big; vector_simp; simpl;
     rewrite (regFitProp ri lti), (regFitProp A ltA);
     reflexivity.
 
   Ltac rjAProof_word :=
     intros pad ri lti A padding;
-    unfold OpcodeDecode; rewrite interpSplit_eval;
+    unfold InstructionDecode; rewrite interpSplit_eval;
     unfold bitvector_fin_big; vector_simp; simpl;
     rewrite (regFitProp ri lti);
     reflexivity.
 
   Ltac AProof_register :=
     intros pad1 pad2 A ltA padding;
-    unfold OpcodeDecode; rewrite interpSplit_eval;
+    unfold InstructionDecode; rewrite interpSplit_eval;
     unfold bitvector_fin_big; vector_simp; simpl;
     rewrite (regFitProp A ltA);
     reflexivity.
 
   Ltac AProof_word :=
     intros pad1 pad2 A padding;
-    unfold OpcodeDecode; rewrite interpSplit_eval;
+    unfold InstructionDecode; rewrite interpSplit_eval;
     unfold bitvector_fin_big; vector_simp; simpl;
     reflexivity.
 
@@ -404,7 +404,7 @@ Module TinyRAMCoding (Params : TinyRAMParameters).
            (A : Word)
            (ltA : proj1_sig (bitvector_fin_big A) < registerCount)
            (padding : Vector.t bool paddingSize),
-    OpcodeDecode (cast (and_code ++ [b0] ++ ri ++ rj ++ padding)
+    InstructionDecode (cast (and_code ++ [b0] ++ ri ++ rj ++ padding)
                        (eq_sym interpSplitLemRight)) A =
     (andI (regFit ri lti) (regFit rj ltj), inr (regFit A ltA)).
   Proof. unfold and_code. rirjAProof_register. Qed.
@@ -415,7 +415,7 @@ Module TinyRAMCoding (Params : TinyRAMParameters).
            (ltj : proj1_sig (bitvector_fin_big rj) < registerCount)
            (A : Word)
            (padding : Vector.t bool paddingSize),
-    OpcodeDecode (cast (and_code ++ [b1] ++ ri ++ rj ++ padding)
+    InstructionDecode (cast (and_code ++ [b1] ++ ri ++ rj ++ padding)
                        (eq_sym interpSplitLemRight)) A =
     (andI (regFit ri lti) (regFit rj ltj), inl A).
   Proof. unfold and_code. rirjAProof_word. Qed.
@@ -429,7 +429,7 @@ Theorem or_decode_register_correct :
            (A : Word)
            (ltA : proj1_sig (bitvector_fin_big A) < registerCount)
            (padding : Vector.t bool paddingSize),
-    OpcodeDecode (cast (or_code ++ [b0] ++ ri ++ rj ++ padding)
+    InstructionDecode (cast (or_code ++ [b0] ++ ri ++ rj ++ padding)
                        (eq_sym interpSplitLemRight)) A =
     (orI (regFit ri lti) (regFit rj ltj), inr (regFit A ltA)).
   Proof. unfold or_code. rirjAProof_register. Qed.
@@ -440,7 +440,7 @@ Theorem or_decode_register_correct :
            (ltj : proj1_sig (bitvector_fin_big rj) < registerCount)
            (A : Word)
            (padding : Vector.t bool paddingSize),
-    OpcodeDecode (cast (or_code ++ [b1] ++ ri ++ rj ++ padding)
+    InstructionDecode (cast (or_code ++ [b1] ++ ri ++ rj ++ padding)
                        (eq_sym interpSplitLemRight)) A =
     (orI (regFit ri lti) (regFit rj ltj), inl A).
   Proof. unfold or_code. rirjAProof_word. Qed.
@@ -454,7 +454,7 @@ Theorem or_decode_register_correct :
            (A : Word)
            (ltA : proj1_sig (bitvector_fin_big A) < registerCount)
            (padding : Vector.t bool paddingSize),
-    OpcodeDecode (cast (xor_code ++ [b0] ++ ri ++ rj ++ padding)
+    InstructionDecode (cast (xor_code ++ [b0] ++ ri ++ rj ++ padding)
                        (eq_sym interpSplitLemRight)) A =
     (xorI (regFit ri lti) (regFit rj ltj), inr (regFit A ltA)).
   Proof. unfold xor_code. rirjAProof_register. Qed.
@@ -465,7 +465,7 @@ Theorem or_decode_register_correct :
            (ltj : proj1_sig (bitvector_fin_big rj) < registerCount)
            (A : Word)
            (padding : Vector.t bool paddingSize),
-    OpcodeDecode (cast (xor_code ++ [b1] ++ ri ++ rj ++ padding)
+    InstructionDecode (cast (xor_code ++ [b1] ++ ri ++ rj ++ padding)
                        (eq_sym interpSplitLemRight)) A =
     (xorI (regFit ri lti) (regFit rj ltj), inl A).
   Proof. unfold xor_code. rirjAProof_word. Qed.
@@ -478,7 +478,7 @@ Theorem or_decode_register_correct :
            (A : Word)
            (ltA : proj1_sig (bitvector_fin_big A) < registerCount)
            (padding : Vector.t bool paddingSize),
-    OpcodeDecode (cast (not_code ++ [b0] ++ ri ++ pad ++ padding)
+    InstructionDecode (cast (not_code ++ [b0] ++ ri ++ pad ++ padding)
                        (eq_sym interpSplitLemRight)) A =
     (notI (regFit ri lti), inr (regFit A ltA)).
   Proof. unfold not_code. riAProof_register. Qed.
@@ -488,7 +488,7 @@ Theorem or_decode_register_correct :
            (lti : proj1_sig (bitvector_fin_big ri) < registerCount)
            (A : Word)
            (padding : Vector.t bool paddingSize),
-    OpcodeDecode (cast (not_code ++ [b1] ++ ri ++ pad ++ padding)
+    InstructionDecode (cast (not_code ++ [b1] ++ ri ++ pad ++ padding)
                        (eq_sym interpSplitLemRight)) A =
     (notI (regFit ri lti), inl A).
   Proof. unfold not_code. riAProof_word. Qed.
@@ -502,7 +502,7 @@ Theorem or_decode_register_correct :
            (A : Word)
            (ltA : proj1_sig (bitvector_fin_big A) < registerCount)
            (padding : Vector.t bool paddingSize),
-    OpcodeDecode (cast (add_code ++ [b0] ++ ri ++ rj ++ padding)
+    InstructionDecode (cast (add_code ++ [b0] ++ ri ++ rj ++ padding)
                        (eq_sym interpSplitLemRight)) A =
     (addI (regFit ri lti) (regFit rj ltj), inr (regFit A ltA)).
   Proof. unfold add_code. rirjAProof_register. Qed.
@@ -513,7 +513,7 @@ Theorem or_decode_register_correct :
            (ltj : proj1_sig (bitvector_fin_big rj) < registerCount)
            (A : Word)
            (padding : Vector.t bool paddingSize),
-    OpcodeDecode (cast (add_code ++ [b1] ++ ri ++ rj ++ padding)
+    InstructionDecode (cast (add_code ++ [b1] ++ ri ++ rj ++ padding)
                        (eq_sym interpSplitLemRight)) A =
     (addI (regFit ri lti) (regFit rj ltj), inl A).
   Proof. unfold add_code. rirjAProof_word. Qed.
@@ -527,7 +527,7 @@ Theorem or_decode_register_correct :
            (A : Word)
            (ltA : proj1_sig (bitvector_fin_big A) < registerCount)
            (padding : Vector.t bool paddingSize),
-    OpcodeDecode (cast (sub_code ++ [b0] ++ ri ++ rj ++ padding)
+    InstructionDecode (cast (sub_code ++ [b0] ++ ri ++ rj ++ padding)
                        (eq_sym interpSplitLemRight)) A =
     (subI (regFit ri lti) (regFit rj ltj), inr (regFit A ltA)).
   Proof. unfold sub_code. rirjAProof_register. Qed.
@@ -538,7 +538,7 @@ Theorem or_decode_register_correct :
            (ltj : proj1_sig (bitvector_fin_big rj) < registerCount)
            (A : Word)
            (padding : Vector.t bool paddingSize),
-    OpcodeDecode (cast (sub_code ++ [b1] ++ ri ++ rj ++ padding)
+    InstructionDecode (cast (sub_code ++ [b1] ++ ri ++ rj ++ padding)
                        (eq_sym interpSplitLemRight)) A =
     (subI (regFit ri lti) (regFit rj ltj), inl A).
   Proof. unfold sub_code. rirjAProof_word. Qed.
@@ -552,7 +552,7 @@ Theorem or_decode_register_correct :
            (A : Word)
            (ltA : proj1_sig (bitvector_fin_big A) < registerCount)
            (padding : Vector.t bool paddingSize),
-    OpcodeDecode (cast (mull_code ++ [b0] ++ ri ++ rj ++ padding)
+    InstructionDecode (cast (mull_code ++ [b0] ++ ri ++ rj ++ padding)
                        (eq_sym interpSplitLemRight)) A =
     (mullI (regFit ri lti) (regFit rj ltj), inr (regFit A ltA)).
   Proof. unfold mull_code. rirjAProof_register. Qed.
@@ -563,7 +563,7 @@ Theorem or_decode_register_correct :
            (ltj : proj1_sig (bitvector_fin_big rj) < registerCount)
            (A : Word)
            (padding : Vector.t bool paddingSize),
-    OpcodeDecode (cast (mull_code ++ [b1] ++ ri ++ rj ++ padding)
+    InstructionDecode (cast (mull_code ++ [b1] ++ ri ++ rj ++ padding)
                        (eq_sym interpSplitLemRight)) A =
     (mullI (regFit ri lti) (regFit rj ltj), inl A).
   Proof. unfold mull_code. rirjAProof_word. Qed.
@@ -577,7 +577,7 @@ Theorem or_decode_register_correct :
            (A : Word)
            (ltA : proj1_sig (bitvector_fin_big A) < registerCount)
            (padding : Vector.t bool paddingSize),
-    OpcodeDecode (cast (umulh_code ++ [b0] ++ ri ++ rj ++ padding)
+    InstructionDecode (cast (umulh_code ++ [b0] ++ ri ++ rj ++ padding)
                        (eq_sym interpSplitLemRight)) A =
     (umulhI (regFit ri lti) (regFit rj ltj), inr (regFit A ltA)).
   Proof. unfold umulh_code. rirjAProof_register. Qed.
@@ -588,7 +588,7 @@ Theorem or_decode_register_correct :
            (ltj : proj1_sig (bitvector_fin_big rj) < registerCount)
            (A : Word)
            (padding : Vector.t bool paddingSize),
-    OpcodeDecode (cast (umulh_code ++ [b1] ++ ri ++ rj ++ padding)
+    InstructionDecode (cast (umulh_code ++ [b1] ++ ri ++ rj ++ padding)
                        (eq_sym interpSplitLemRight)) A =
     (umulhI (regFit ri lti) (regFit rj ltj), inl A).
   Proof. unfold umulh_code. rirjAProof_word. Qed.
@@ -602,7 +602,7 @@ Theorem or_decode_register_correct :
            (A : Word)
            (ltA : proj1_sig (bitvector_fin_big A) < registerCount)
            (padding : Vector.t bool paddingSize),
-    OpcodeDecode (cast (smulh_code ++ [b0] ++ ri ++ rj ++ padding)
+    InstructionDecode (cast (smulh_code ++ [b0] ++ ri ++ rj ++ padding)
                        (eq_sym interpSplitLemRight)) A =
     (smulhI (regFit ri lti) (regFit rj ltj), inr (regFit A ltA)).
   Proof. unfold smulh_code. rirjAProof_register. Qed.
@@ -613,7 +613,7 @@ Theorem or_decode_register_correct :
            (ltj : proj1_sig (bitvector_fin_big rj) < registerCount)
            (A : Word)
            (padding : Vector.t bool paddingSize),
-    OpcodeDecode (cast (smulh_code ++ [b1] ++ ri ++ rj ++ padding)
+    InstructionDecode (cast (smulh_code ++ [b1] ++ ri ++ rj ++ padding)
                        (eq_sym interpSplitLemRight)) A =
     (smulhI (regFit ri lti) (regFit rj ltj), inl A).
   Proof. unfold smulh_code. rirjAProof_word. Qed.
@@ -627,7 +627,7 @@ Theorem or_decode_register_correct :
            (A : Word)
            (ltA : proj1_sig (bitvector_fin_big A) < registerCount)
            (padding : Vector.t bool paddingSize),
-    OpcodeDecode (cast (udiv_code ++ [b0] ++ ri ++ rj ++ padding)
+    InstructionDecode (cast (udiv_code ++ [b0] ++ ri ++ rj ++ padding)
                        (eq_sym interpSplitLemRight)) A =
     (udivI (regFit ri lti) (regFit rj ltj), inr (regFit A ltA)).
   Proof. unfold udiv_code. rirjAProof_register. Qed.
@@ -638,7 +638,7 @@ Theorem or_decode_register_correct :
            (ltj : proj1_sig (bitvector_fin_big rj) < registerCount)
            (A : Word)
            (padding : Vector.t bool paddingSize),
-    OpcodeDecode (cast (udiv_code ++ [b1] ++ ri ++ rj ++ padding)
+    InstructionDecode (cast (udiv_code ++ [b1] ++ ri ++ rj ++ padding)
                        (eq_sym interpSplitLemRight)) A =
     (udivI (regFit ri lti) (regFit rj ltj), inl A).
   Proof. unfold udiv_code. rirjAProof_word. Qed.
@@ -652,7 +652,7 @@ Theorem or_decode_register_correct :
            (A : Word)
            (ltA : proj1_sig (bitvector_fin_big A) < registerCount)
            (padding : Vector.t bool paddingSize),
-    OpcodeDecode (cast (umod_code ++ [b0] ++ ri ++ rj ++ padding)
+    InstructionDecode (cast (umod_code ++ [b0] ++ ri ++ rj ++ padding)
                        (eq_sym interpSplitLemRight)) A =
     (umodI (regFit ri lti) (regFit rj ltj), inr (regFit A ltA)).
   Proof. unfold umod_code. rirjAProof_register. Qed.
@@ -663,7 +663,7 @@ Theorem or_decode_register_correct :
            (ltj : proj1_sig (bitvector_fin_big rj) < registerCount)
            (A : Word)
            (padding : Vector.t bool paddingSize),
-    OpcodeDecode (cast (umod_code ++ [b1] ++ ri ++ rj ++ padding)
+    InstructionDecode (cast (umod_code ++ [b1] ++ ri ++ rj ++ padding)
                        (eq_sym interpSplitLemRight)) A =
     (umodI (regFit ri lti) (regFit rj ltj), inl A).
   Proof. unfold umod_code. rirjAProof_word. Qed.
@@ -677,7 +677,7 @@ Theorem or_decode_register_correct :
            (A : Word)
            (ltA : proj1_sig (bitvector_fin_big A) < registerCount)
            (padding : Vector.t bool paddingSize),
-    OpcodeDecode (cast (shl_code ++ [b0] ++ ri ++ rj ++ padding)
+    InstructionDecode (cast (shl_code ++ [b0] ++ ri ++ rj ++ padding)
                        (eq_sym interpSplitLemRight)) A =
     (shlI (regFit ri lti) (regFit rj ltj), inr (regFit A ltA)).
   Proof. unfold shl_code. rirjAProof_register. Qed.
@@ -688,7 +688,7 @@ Theorem or_decode_register_correct :
            (ltj : proj1_sig (bitvector_fin_big rj) < registerCount)
            (A : Word)
            (padding : Vector.t bool paddingSize),
-    OpcodeDecode (cast (shl_code ++ [b1] ++ ri ++ rj ++ padding)
+    InstructionDecode (cast (shl_code ++ [b1] ++ ri ++ rj ++ padding)
                        (eq_sym interpSplitLemRight)) A =
     (shlI (regFit ri lti) (regFit rj ltj), inl A).
   Proof. unfold shl_code. rirjAProof_word. Qed.
@@ -702,7 +702,7 @@ Theorem or_decode_register_correct :
            (A : Word)
            (ltA : proj1_sig (bitvector_fin_big A) < registerCount)
            (padding : Vector.t bool paddingSize),
-    OpcodeDecode (cast (shr_code ++ [b0] ++ ri ++ rj ++ padding)
+    InstructionDecode (cast (shr_code ++ [b0] ++ ri ++ rj ++ padding)
                        (eq_sym interpSplitLemRight)) A =
     (shrI (regFit ri lti) (regFit rj ltj), inr (regFit A ltA)).
   Proof. unfold shr_code. rirjAProof_register. Qed.
@@ -713,7 +713,7 @@ Theorem or_decode_register_correct :
            (ltj : proj1_sig (bitvector_fin_big rj) < registerCount)
            (A : Word)
            (padding : Vector.t bool paddingSize),
-    OpcodeDecode (cast (shr_code ++ [b1] ++ ri ++ rj ++ padding)
+    InstructionDecode (cast (shr_code ++ [b1] ++ ri ++ rj ++ padding)
                        (eq_sym interpSplitLemRight)) A =
     (shrI (regFit ri lti) (regFit rj ltj), inl A).
   Proof. unfold shr_code. rirjAProof_word. Qed.
@@ -726,7 +726,7 @@ Theorem or_decode_register_correct :
            (A : Word)
            (ltA : proj1_sig (bitvector_fin_big A) < registerCount)
            (padding : Vector.t bool paddingSize),
-    OpcodeDecode (cast (cmpe_code ++ [b0] ++ pad ++ ri ++ padding)
+    InstructionDecode (cast (cmpe_code ++ [b0] ++ pad ++ ri ++ padding)
                        (eq_sym interpSplitLemRight)) A =
     (cmpeI (regFit ri lti), inr (regFit A ltA)).
   Proof. unfold cmpe_code. rjAProof_register. Qed.
@@ -736,7 +736,7 @@ Theorem or_decode_register_correct :
            (lti : proj1_sig (bitvector_fin_big ri) < registerCount)
            (A : Word)
            (padding : Vector.t bool paddingSize),
-    OpcodeDecode (cast (cmpe_code ++ [b1] ++ pad ++ ri ++ padding)
+    InstructionDecode (cast (cmpe_code ++ [b1] ++ pad ++ ri ++ padding)
                        (eq_sym interpSplitLemRight)) A =
     (cmpeI (regFit ri lti), inl A).
   Proof. unfold cmpe_code. rjAProof_word. Qed.
@@ -749,7 +749,7 @@ Theorem or_decode_register_correct :
            (A : Word)
            (ltA : proj1_sig (bitvector_fin_big A) < registerCount)
            (padding : Vector.t bool paddingSize),
-    OpcodeDecode (cast (cmpa_code ++ [b0] ++ pad ++ ri ++ padding)
+    InstructionDecode (cast (cmpa_code ++ [b0] ++ pad ++ ri ++ padding)
                        (eq_sym interpSplitLemRight)) A =
     (cmpaI (regFit ri lti), inr (regFit A ltA)).
   Proof. unfold cmpa_code. rjAProof_register. Qed.
@@ -759,7 +759,7 @@ Theorem or_decode_register_correct :
            (lti : proj1_sig (bitvector_fin_big ri) < registerCount)
            (A : Word)
            (padding : Vector.t bool paddingSize),
-    OpcodeDecode (cast (cmpa_code ++ [b1] ++ pad ++ ri ++ padding)
+    InstructionDecode (cast (cmpa_code ++ [b1] ++ pad ++ ri ++ padding)
                        (eq_sym interpSplitLemRight)) A =
     (cmpaI (regFit ri lti), inl A).
   Proof. unfold cmpa_code. rjAProof_word. Qed.
@@ -772,7 +772,7 @@ Theorem or_decode_register_correct :
            (A : Word)
            (ltA : proj1_sig (bitvector_fin_big A) < registerCount)
            (padding : Vector.t bool paddingSize),
-    OpcodeDecode (cast (cmpae_code ++ [b0] ++ pad ++ ri ++ padding)
+    InstructionDecode (cast (cmpae_code ++ [b0] ++ pad ++ ri ++ padding)
                        (eq_sym interpSplitLemRight)) A =
     (cmpaeI (regFit ri lti), inr (regFit A ltA)).
   Proof. unfold cmpae_code. rjAProof_register. Qed.
@@ -782,7 +782,7 @@ Theorem or_decode_register_correct :
            (lti : proj1_sig (bitvector_fin_big ri) < registerCount)
            (A : Word)
            (padding : Vector.t bool paddingSize),
-    OpcodeDecode (cast (cmpae_code ++ [b1] ++ pad ++ ri ++ padding)
+    InstructionDecode (cast (cmpae_code ++ [b1] ++ pad ++ ri ++ padding)
                        (eq_sym interpSplitLemRight)) A =
     (cmpaeI (regFit ri lti), inl A).
   Proof. unfold cmpae_code. rjAProof_word. Qed.
@@ -795,7 +795,7 @@ Theorem or_decode_register_correct :
            (A : Word)
            (ltA : proj1_sig (bitvector_fin_big A) < registerCount)
            (padding : Vector.t bool paddingSize),
-    OpcodeDecode (cast (cmpg_code ++ [b0] ++ pad ++ ri ++ padding)
+    InstructionDecode (cast (cmpg_code ++ [b0] ++ pad ++ ri ++ padding)
                        (eq_sym interpSplitLemRight)) A =
     (cmpgI (regFit ri lti), inr (regFit A ltA)).
   Proof. unfold cmpg_code. rjAProof_register. Qed.
@@ -805,7 +805,7 @@ Theorem or_decode_register_correct :
            (lti : proj1_sig (bitvector_fin_big ri) < registerCount)
            (A : Word)
            (padding : Vector.t bool paddingSize),
-    OpcodeDecode (cast (cmpg_code ++ [b1] ++ pad ++ ri ++ padding)
+    InstructionDecode (cast (cmpg_code ++ [b1] ++ pad ++ ri ++ padding)
                        (eq_sym interpSplitLemRight)) A =
     (cmpgI (regFit ri lti), inl A).
   Proof. unfold cmpg_code. rjAProof_word. Qed.
@@ -818,7 +818,7 @@ Theorem or_decode_register_correct :
            (A : Word)
            (ltA : proj1_sig (bitvector_fin_big A) < registerCount)
            (padding : Vector.t bool paddingSize),
-    OpcodeDecode (cast (cmpge_code ++ [b0] ++ pad ++ ri ++ padding)
+    InstructionDecode (cast (cmpge_code ++ [b0] ++ pad ++ ri ++ padding)
                        (eq_sym interpSplitLemRight)) A =
     (cmpgeI (regFit ri lti), inr (regFit A ltA)).
   Proof. unfold cmpge_code. rjAProof_register. Qed.
@@ -828,7 +828,7 @@ Theorem or_decode_register_correct :
            (lti : proj1_sig (bitvector_fin_big ri) < registerCount)
            (A : Word)
            (padding : Vector.t bool paddingSize),
-    OpcodeDecode (cast (cmpge_code ++ [b1] ++ pad ++ ri ++ padding)
+    InstructionDecode (cast (cmpge_code ++ [b1] ++ pad ++ ri ++ padding)
                        (eq_sym interpSplitLemRight)) A =
     (cmpgeI (regFit ri lti), inl A).
   Proof. unfold cmpge_code. rjAProof_word. Qed.
@@ -841,7 +841,7 @@ Theorem or_decode_register_correct :
            (A : Word)
            (ltA : proj1_sig (bitvector_fin_big A) < registerCount)
            (padding : Vector.t bool paddingSize),
-    OpcodeDecode (cast (mov_code ++ [b0] ++ ri ++ pad ++ padding)
+    InstructionDecode (cast (mov_code ++ [b0] ++ ri ++ pad ++ padding)
                        (eq_sym interpSplitLemRight)) A =
     (movI (regFit ri lti), inr (regFit A ltA)).
   Proof. unfold mov_code. riAProof_register. Qed.
@@ -851,7 +851,7 @@ Theorem or_decode_register_correct :
            (lti : proj1_sig (bitvector_fin_big ri) < registerCount)
            (A : Word)
            (padding : Vector.t bool paddingSize),
-    OpcodeDecode (cast (mov_code ++ [b1] ++ ri ++ pad ++ padding)
+    InstructionDecode (cast (mov_code ++ [b1] ++ ri ++ pad ++ padding)
                        (eq_sym interpSplitLemRight)) A =
     (movI (regFit ri lti), inl A).
   Proof. unfold mov_code. riAProof_word. Qed.
@@ -864,7 +864,7 @@ Theorem or_decode_register_correct :
            (A : Word)
            (ltA : proj1_sig (bitvector_fin_big A) < registerCount)
            (padding : Vector.t bool paddingSize),
-    OpcodeDecode (cast (cmov_code ++ [b0] ++ ri ++ pad ++ padding)
+    InstructionDecode (cast (cmov_code ++ [b0] ++ ri ++ pad ++ padding)
                        (eq_sym interpSplitLemRight)) A =
     (cmovI (regFit ri lti), inr (regFit A ltA)).
   Proof. unfold cmov_code. riAProof_register. Qed.
@@ -874,7 +874,7 @@ Theorem or_decode_register_correct :
            (lti : proj1_sig (bitvector_fin_big ri) < registerCount)
            (A : Word)
            (padding : Vector.t bool paddingSize),
-    OpcodeDecode (cast (cmov_code ++ [b1] ++ ri ++ pad ++ padding)
+    InstructionDecode (cast (cmov_code ++ [b1] ++ ri ++ pad ++ padding)
                        (eq_sym interpSplitLemRight)) A =
     (cmovI (regFit ri lti), inl A).
   Proof. unfold cmov_code. riAProof_word. Qed.
@@ -886,7 +886,7 @@ Theorem or_decode_register_correct :
            (A : Word)
            (ltA : proj1_sig (bitvector_fin_big A) < registerCount)
            (padding : Vector.t bool paddingSize),
-    OpcodeDecode (cast (jmp_code ++ [b0] ++ pad1 ++ pad2 ++ padding)
+    InstructionDecode (cast (jmp_code ++ [b0] ++ pad1 ++ pad2 ++ padding)
                        (eq_sym interpSplitLemRight)) A =
     (jmpI, inr (regFit A ltA)).
   Proof. unfold jmp_code. AProof_register. Qed.
@@ -895,7 +895,7 @@ Theorem or_decode_register_correct :
     forall (pad1 pad2 : Vector.t bool (log2_up registerCount))
            (A : Word)
            (padding : Vector.t bool paddingSize),
-    OpcodeDecode (cast (jmp_code ++ [b1] ++ pad1 ++ pad2 ++ padding)
+    InstructionDecode (cast (jmp_code ++ [b1] ++ pad1 ++ pad2 ++ padding)
                        (eq_sym interpSplitLemRight)) A =
     (jmpI, inl A).
   Proof. unfold jmp_code. AProof_word. Qed.
@@ -907,7 +907,7 @@ Theorem or_decode_register_correct :
            (A : Word)
            (ltA : proj1_sig (bitvector_fin_big A) < registerCount)
            (padding : Vector.t bool paddingSize),
-    OpcodeDecode (cast (cjmp_code ++ [b0] ++ pad1 ++ pad2 ++ padding)
+    InstructionDecode (cast (cjmp_code ++ [b0] ++ pad1 ++ pad2 ++ padding)
                        (eq_sym interpSplitLemRight)) A =
     (cjmpI, inr (regFit A ltA)).
   Proof. unfold cjmp_code. AProof_register. Qed.
@@ -916,7 +916,7 @@ Theorem or_decode_register_correct :
     forall (pad1 pad2 : Vector.t bool (log2_up registerCount))
            (A : Word)
            (padding : Vector.t bool paddingSize),
-    OpcodeDecode (cast (cjmp_code ++ [b1] ++ pad1 ++ pad2 ++ padding)
+    InstructionDecode (cast (cjmp_code ++ [b1] ++ pad1 ++ pad2 ++ padding)
                        (eq_sym interpSplitLemRight)) A =
     (cjmpI, inl A).
   Proof. unfold cjmp_code. AProof_word. Qed.
@@ -928,7 +928,7 @@ Theorem or_decode_register_correct :
            (A : Word)
            (ltA : proj1_sig (bitvector_fin_big A) < registerCount)
            (padding : Vector.t bool paddingSize),
-    OpcodeDecode (cast (cnjmp_code ++ [b0] ++ pad1 ++ pad2 ++ padding)
+    InstructionDecode (cast (cnjmp_code ++ [b0] ++ pad1 ++ pad2 ++ padding)
                        (eq_sym interpSplitLemRight)) A =
     (cnjmpI, inr (regFit A ltA)).
   Proof. unfold cnjmp_code. AProof_register. Qed.
@@ -937,7 +937,7 @@ Theorem or_decode_register_correct :
     forall (pad1 pad2 : Vector.t bool (log2_up registerCount))
            (A : Word)
            (padding : Vector.t bool paddingSize),
-    OpcodeDecode (cast (cnjmp_code ++ [b1] ++ pad1 ++ pad2 ++ padding)
+    InstructionDecode (cast (cnjmp_code ++ [b1] ++ pad1 ++ pad2 ++ padding)
                        (eq_sym interpSplitLemRight)) A =
     (cnjmpI, inl A).
   Proof. unfold cnjmp_code. AProof_word. Qed.
@@ -950,7 +950,7 @@ Theorem or_decode_register_correct :
            (A : Word)
            (ltA : proj1_sig (bitvector_fin_big A) < registerCount)
            (padding : Vector.t bool paddingSize),
-    OpcodeDecode (cast (store_b_code ++ [b0] ++ ri ++ pad ++ padding)
+    InstructionDecode (cast (store_b_code ++ [b0] ++ ri ++ pad ++ padding)
                        (eq_sym interpSplitLemRight)) A =
     (store_bI (regFit ri lti), inr (regFit A ltA)).
   Proof. unfold store_b_code. riAProof_register. Qed.
@@ -960,7 +960,7 @@ Theorem or_decode_register_correct :
            (lti : proj1_sig (bitvector_fin_big ri) < registerCount)
            (A : Word)
            (padding : Vector.t bool paddingSize),
-    OpcodeDecode (cast (store_b_code ++ [b1] ++ ri ++ pad ++ padding)
+    InstructionDecode (cast (store_b_code ++ [b1] ++ ri ++ pad ++ padding)
                        (eq_sym interpSplitLemRight)) A =
     (store_bI (regFit ri lti), inl A).
   Proof. unfold store_b_code. riAProof_word. Qed.
@@ -973,7 +973,7 @@ Theorem or_decode_register_correct :
            (A : Word)
            (ltA : proj1_sig (bitvector_fin_big A) < registerCount)
            (padding : Vector.t bool paddingSize),
-    OpcodeDecode (cast (load_b_code ++ [b0] ++ ri ++ pad ++ padding)
+    InstructionDecode (cast (load_b_code ++ [b0] ++ ri ++ pad ++ padding)
                        (eq_sym interpSplitLemRight)) A =
     (load_bI (regFit ri lti), inr (regFit A ltA)).
   Proof. unfold load_b_code. riAProof_register. Qed.
@@ -983,7 +983,7 @@ Theorem or_decode_register_correct :
            (lti : proj1_sig (bitvector_fin_big ri) < registerCount)
            (A : Word)
            (padding : Vector.t bool paddingSize),
-    OpcodeDecode (cast (load_b_code ++ [b1] ++ ri ++ pad ++ padding)
+    InstructionDecode (cast (load_b_code ++ [b1] ++ ri ++ pad ++ padding)
                        (eq_sym interpSplitLemRight)) A =
     (load_bI (regFit ri lti), inl A).
   Proof. unfold load_b_code. riAProof_word. Qed.
@@ -996,7 +996,7 @@ Theorem or_decode_register_correct :
            (A : Word)
            (ltA : proj1_sig (bitvector_fin_big A) < registerCount)
            (padding : Vector.t bool paddingSize),
-    OpcodeDecode (cast (store_w_code ++ [b0] ++ ri ++ pad ++ padding)
+    InstructionDecode (cast (store_w_code ++ [b0] ++ ri ++ pad ++ padding)
                        (eq_sym interpSplitLemRight)) A =
     (store_wI (regFit ri lti), inr (regFit A ltA)).
   Proof. unfold store_w_code. riAProof_register. Qed.
@@ -1006,7 +1006,7 @@ Theorem or_decode_register_correct :
            (lti : proj1_sig (bitvector_fin_big ri) < registerCount)
            (A : Word)
            (padding : Vector.t bool paddingSize),
-    OpcodeDecode (cast (store_w_code ++ [b1] ++ ri ++ pad ++ padding)
+    InstructionDecode (cast (store_w_code ++ [b1] ++ ri ++ pad ++ padding)
                        (eq_sym interpSplitLemRight)) A =
     (store_wI (regFit ri lti), inl A).
   Proof. unfold store_w_code. riAProof_word. Qed.
@@ -1019,7 +1019,7 @@ Theorem or_decode_register_correct :
            (A : Word)
            (ltA : proj1_sig (bitvector_fin_big A) < registerCount)
            (padding : Vector.t bool paddingSize),
-    OpcodeDecode (cast (load_w_code ++ [b0] ++ ri ++ pad ++ padding)
+    InstructionDecode (cast (load_w_code ++ [b0] ++ ri ++ pad ++ padding)
                        (eq_sym interpSplitLemRight)) A =
     (load_wI (regFit ri lti), inr (regFit A ltA)).
   Proof. unfold load_w_code. riAProof_register. Qed.
@@ -1029,7 +1029,7 @@ Theorem or_decode_register_correct :
            (lti : proj1_sig (bitvector_fin_big ri) < registerCount)
            (A : Word)
            (padding : Vector.t bool paddingSize),
-    OpcodeDecode (cast (load_w_code ++ [b1] ++ ri ++ pad ++ padding)
+    InstructionDecode (cast (load_w_code ++ [b1] ++ ri ++ pad ++ padding)
                        (eq_sym interpSplitLemRight)) A =
     (load_wI (regFit ri lti), inl A).
   Proof. unfold load_w_code. riAProof_word. Qed.
@@ -1042,7 +1042,7 @@ Theorem or_decode_register_correct :
            (A : Word)
            (ltA : proj1_sig (bitvector_fin_big A) < registerCount)
            (padding : Vector.t bool paddingSize),
-    OpcodeDecode (cast (read_code ++ [b0] ++ ri ++ pad ++ padding)
+    InstructionDecode (cast (read_code ++ [b0] ++ ri ++ pad ++ padding)
                        (eq_sym interpSplitLemRight)) A =
     (readI (regFit ri lti), inr (regFit A ltA)).
   Proof. unfold read_code. riAProof_register. Qed.
@@ -1052,7 +1052,7 @@ Theorem or_decode_register_correct :
            (lti : proj1_sig (bitvector_fin_big ri) < registerCount)
            (A : Word)
            (padding : Vector.t bool paddingSize),
-    OpcodeDecode (cast (read_code ++ [b1] ++ ri ++ pad ++ padding)
+    InstructionDecode (cast (read_code ++ [b1] ++ ri ++ pad ++ padding)
                        (eq_sym interpSplitLemRight)) A =
     (readI (regFit ri lti), inl A).
   Proof. unfold read_code. riAProof_word. Qed.
@@ -1064,7 +1064,7 @@ Theorem or_decode_register_correct :
            (A : Word)
            (ltA : proj1_sig (bitvector_fin_big A) < registerCount)
            (padding : Vector.t bool paddingSize),
-    OpcodeDecode (cast (answer_code ++ [b0] ++ pad1 ++ pad2 ++ padding)
+    InstructionDecode (cast (answer_code ++ [b0] ++ pad1 ++ pad2 ++ padding)
                        (eq_sym interpSplitLemRight)) A =
     (answerI, inr (regFit A ltA)).
   Proof. unfold answer_code. AProof_register. Qed.
@@ -1073,7 +1073,7 @@ Theorem or_decode_register_correct :
     forall (pad1 pad2 : Vector.t bool (log2_up registerCount))
            (A : Word)
            (padding : Vector.t bool paddingSize),
-    OpcodeDecode (cast (answer_code ++ [b1] ++ pad1 ++ pad2 ++ padding)
+    InstructionDecode (cast (answer_code ++ [b1] ++ pad1 ++ pad2 ++ padding)
                        (eq_sym interpSplitLemRight)) A =
     (answerI, inl A).
   Proof. unfold answer_code. AProof_word. Qed.
@@ -1099,7 +1099,7 @@ Theorem or_decode_register_correct :
     rewrite PeanoNat.Nat.log2_up_le_pow2; lia.
   Defined.
 
-  Definition OpcodeEncode (o : Opcode) : Word * Word :=
+  Definition InstructionEncode (o : Instruction) : Word * Word :=
     match o with
     | (andI ri rj, op) =>
       (cast (and_code ++ [option_bool op] ++ reg_vect ri ++ reg_vect rj ++ const b0 _)
@@ -1255,10 +1255,10 @@ Theorem or_decode_register_correct :
     rewrite rDef in H.
 
   Theorem encode_decode_id : forall o, 
-    uncurry OpcodeDecode (OpcodeEncode o) = o.
+    uncurry InstructionDecode (InstructionEncode o) = o.
   Proof.
     intro o; destruct o as [o op]; destruct o;
-    unfold OpcodeEncode, uncurry;
+    unfold InstructionEncode, uncurry;
     destruct op; unfold option_bool;
     try (destruct r as [r' rprp] eqn:rDef);
     try (destruct r0 as [r0' r0prp] eqn:r0Def);
